Preliminary work on using WF relation

src/theory/abstract_hoare_logic/abstract_hoare_logicScript.sml
@@ -134,69 +134,178 @@ REPEAT STRIP_TAC >>
 METIS_TAC [weak_unique_thm]
 );
 
-
-
-val loop_step_def = Define `
-  loop_step m ms var l le invariant C1 =
+(*
+val weak_loop_step_def = Define `
+  weak_loop_step m ms var l le invariant C1 =
     let x:num = var ms in
-    (\ms'. m.weak ms ({l} UNION le) ms' /\
-	   (invariant ms /\ C1 ms) /\
-	   ((m.pc ms' = l) /\ invariant ms' /\ (var ms' < x) /\ (var ms' >= 0))
-    )
+      (\ms'. m.weak ms ({l} UNION le) ms' /\
+             (invariant ms /\ C1 ms) /\
+             ((m.pc ms' = l) /\ invariant ms' /\ (var ms' < x) /\ (var ms' >= 0))
+      )
 `;
+*)
 
+(* TODO: Address minimum? (var ms' >= 0)
+ *       Should this have assumption "WF wf_rel"?*)
+
+val weak_loop_step_def = Define `
+  weak_loop_step m ms wf_rel var l le invariant C1 =
+    let x = var ms in
+      (\ms'. (*(WF wf_rel) ==> *) (WF wf_rel) /\
+             m.weak ms ({l} UNION le) ms' /\
+             (invariant ms /\ C1 ms) /\
+             ((m.pc ms' = l) /\ invariant ms' /\ (wf_rel (var ms') x))
+      )
+`;
+(*
 val loop_fun_defn =
   Hol_defn "loop_fun" `
-    loop_fun m ms var l le invariant C1  =
-      let MS' = loop_step m ms var l le invariant C1 in
-      if MS' = {} then ms
-      else let ms' = (CHOICE MS') in
-	(loop_fun m ms' var l le invariant C1)
+    loop_fun m ms wf_rel var l le invariant C1  =
+      let MS' = weak_loop_step m ms wf_rel var l le invariant C1 in
+        if MS' = {}
+        then ms
+	else let ms' = (CHOICE MS') in
+	       (loop_fun m ms' wf_rel var l le invariant C1)
 `;
-
-(*
+*)
+(* For debugging:
 Defn.tgoal loop_fun_defn
 *)
-val (loop_fun_eqns, loop_fun_ind) = Defn.tprove(loop_fun_defn,
-  FULL_SIMP_TAC std_ss [loop_step_def] >>
-  WF_REL_TAC `measure (\(m,ms,var,l,le,invariant,C1). var ms)` >>
-  REPEAT STRIP_TAC >>
+(*
+``?R'.
+       WF R' /\
+       !C1 invariant le l wf_rel var ms m MS' ms'.
+           (MS' = weak_loop_step m ms wf_rel var l le invariant C1) /\
+           MS' <> {} /\ (ms' = CHOICE MS') ==>
+           R' (m,ms',wf_rel,var,l,le,invariant,C1)
+             (m,ms,wf_rel,var,l,le,invariant,C1)``
+
+REPEAT STRIP_TAC >>
+FULL_SIMP_TAC std_ss [weak_loop_step_def] >>
+Q.EXISTS_TAC `\(m, ms,wf_rel,var,l,le,invariant,C1) (m, ms',wf_rel,var,l,le,invariant,C1). wf_rel  (var ms) (var ms')` >>
+REPEAT STRIP_TAC >| [
+  (* This we need to have as assumption... *)
+Q.EXISTS_TAC `\(m, ms,wf_rel',var,l,le,invariant,C1) (m, ms',wf_rel',var,l,le,invariant,C1). wf_rel (var ms) (var ms')` >>
+  cheat,
+
+  (* From assumption to be added... *)
   REV_FULL_SIMP_TAC std_ss [LET_DEF] >>
+  FULL_SIMP_TAC std_ss [] >>
   Q.ABBREV_TAC `MS' =  (\ms'.
-               m.weak ms ({l} UNION le) ms' /\ (invariant ms /\ C1 ms) /\
-               ((m.pc ms') = l) /\ invariant ms' /\ var ms' < var ms)` >>
+	       WF wf_rel /\ m.weak ms ({l} UNION le) ms' /\ (invariant ms /\ C1 ms) /\
+	       ((m.pc ms') = l) /\ invariant ms' /\ wf_rel (var ms') (var ms))` >>
   ASSUME_TAC (ISPEC ``MS':'a->bool`` pred_setTheory.CHOICE_DEF)  >>
   REV_FULL_SIMP_TAC std_ss [] >>
   FULL_SIMP_TAC std_ss [Abbr `MS'`, pred_setTheory.IN_ABS]
+]
+*)
+(* TODO: Look at the resulting loop_fun_ind, see if you can prove it separately...*)
+val loop_fun_ind = prove(
+``!P.
+  (!m ms wf_rel var l le invariant C1.
+       (!MS' ms'.
+	    (MS' = weak_loop_step m ms wf_rel var l le invariant C1) /\
+	    MS' <> {} /\ (ms' = CHOICE MS') ==>
+	    P m ms' wf_rel var l le invariant C1) ==>
+       P m ms wf_rel var l le invariant C1) ==>
+  !v v1 v2 v3 v4 v5 v6 v7. P v v1 v2 v3 v4 v5 v6 v7``,
+
+REPEAT STRIP_TAC >>
+FULL_SIMP_TAC std_ss [weak_loop_step_def] >>
+QSPECL_X_ASSUM ``!m. _`` [`v`, `v1`, `v2`, `v3`, `v4`, `v5`, `v6`, `v7`] >>
+Cases_on `WF v2` >>
+  REV_FULL_SIMP_TAC std_ss [LET_DEF] >>
+
+  Q.ABBREV_TAC `MS' =  (λms'.
+          WF v2 ∧ v.weak v1 ({v4} ∪ v5) ms' ∧ (v6 v1 ∧ v7 v1) ∧
+          (v.pc ms' = v4) ∧ v6 ms' ∧ v2 (v3 ms') (v3 v1))` >>
+ ASSUME_TAC (ISPEC ``MS':'a->bool`` pred_setTheory.CHOICE_DEF)  >>
+  subgoal `MS' <> {}` >- (
+    cheat
+  ) >>
+FULL_SIMP_TAC std_ss [] >>
+cheat
 );
 
 
+
+(*
+val (loop_fun_eqns, loop_fun_ind) =
+  Defn.tprove(loop_fun_defn,
+
+FULL_SIMP_TAC std_ss [weak_loop_step_def] >>
+Q.EXISTS_TAC `\(m, ms,wf_rel,var,l,le,invariant,C1) (m, ms',wf_rel,var,l,le,invariant,C1). wf_rel (var ms) (var ms')` >>
+REPEAT STRIP_TAC >| [
+  (* This we need to have as assumption... *)
+  cheat,
+
+  (* From assumption to be added... *)
+  subgoal `WF wf_rel` >- (
+    cheat
+  ) >>
+  REV_FULL_SIMP_TAC std_ss [LET_DEF] >>
+  FULL_SIMP_TAC std_ss [] >>
+  Q.ABBREV_TAC `MS' =  (\ms'.
+	       m.weak ms ({l} UNION le) ms' /\ (invariant ms /\ C1 ms) /\
+	       ((m.pc ms') = l) /\ invariant ms' /\ wf_rel (var ms') (var ms))` >>
+  ASSUME_TAC (ISPEC ``MS':'a->bool`` pred_setTheory.CHOICE_DEF)  >>
+  REV_FULL_SIMP_TAC std_ss [] >>
+  FULL_SIMP_TAC std_ss [Abbr `MS'`, pred_setTheory.IN_ABS]
+]
+);
+*)
+
 val abstract_loop_jgmt_def = Define `
-  abstract_loop_jgmt m l le invariant C1 var =
-    (~(l IN le) /\
-    !x. abstract_jgmt m l ({l} UNION le) (\ms. invariant ms /\ C1 ms /\ var ms = x:num)
-          (\ms. m.pc ms = l /\ invariant ms /\ var ms < x /\ var ms >= 0))
+  abstract_loop_jgmt m l le invariant C1 wf_rel var =
+    l NOTIN le /\ WF wf_rel /\
+    (!x. (abstract_jgmt m l ({l} UNION le) (\ms. invariant ms /\ C1 ms /\ (var ms = x))
+         (\ms. (m.pc ms = l) /\ invariant ms /\ (wf_rel (var ms) x))))
 `;
 
 (* Note that due to loop_fun_ind relating states ms and ms' at loop points,
  * ms needs to be exposed also here. Either this can be explicitly specified
  * in the precondition of the conclusion, or the definition can be unfolded, like here *)
 val loop_fun_ind_spec =
-  Q.SPEC `\m ms var l le invariant C1.
+  Q.SPEC `\m ms wf_rel var l le invariant C1.
 	   weak_model m ==>
-	   abstract_loop_jgmt m l le invariant C1 var ==>
+           WF wf_rel ==>
+	   abstract_loop_jgmt m l le invariant C1 wf_rel var ==>
 	   abstract_jgmt m l le (\ms. invariant ms /\ ~C1 ms) post ==>
-	   (invariant ms /\ m.pc ms = l) ==>
+	   (invariant ms /\ (m.pc ms = l) /\ C1 ms) ==>
 	   (?ms'. m.weak ms le ms' /\ post ms')` loop_fun_ind;
 
 
+(*
+   ``!m ms wf_rel var l le invariant C1.
+         (!MS' ms'.
+              (MS' = weak_loop_step m ms wf_rel var l le invariant C1) /\
+              MS' <> {} /\ (ms' = CHOICE MS') ==>
+              (\m ms wf_rel var l le invariant C1.
+                   weak_model m ==>
+                   WF wf_rel ==>
+                   abstract_loop_jgmt m l le invariant C1 wf_rel var ==>
+                   weak_triple m l le (\ms. invariant ms /\ ~C1 ms) post ==>
+                   invariant ms /\ (m.pc ms = l) /\ C1 ms ==>
+                   ?ms'. m.weak ms le ms' /\ post ms') m ms' wf_rel var l le
+                invariant C1) ==>
+         (\m ms wf_rel var l le invariant C1.
+              weak_model m ==>
+              WF wf_rel ==>
+              abstract_loop_jgmt m l le invariant C1 wf_rel var ==>
+              weak_triple m l le (\ms. invariant ms /\ ~C1 ms) post ==>
+              invariant ms /\ (m.pc ms = l) /\ C1 ms ==>
+              ?ms'. m.weak ms le ms' /\ post ms') m ms wf_rel var l le
+           invariant C1``
+*)
+
 val inductive_invariant_goal = fst $ dest_imp $ concl loop_fun_ind_spec;
 
-
+(* Below is still TODO... *)
 val inductive_invariant = prove(``
-  ^inductive_invariant_goal
+^inductive_invariant_goal
 ``,
 
+(* New proof without wf_rel:
 rpt strip_tac >>
 fs [] >>
 rpt strip_tac >>
@@ -245,20 +354,111 @@ qexistsl_tac [`{l}`, `ms'`] >>
 Q.SUBGOAL_THEN `l NOTIN le` (fn thm => fs [thm]) >- (
   fs [abstract_loop_jgmt_def, pred_setTheory.IN_SING]
 )
+*)
+REPEAT STRIP_TAC >>
+FULL_SIMP_TAC std_ss [] >>
+REPEAT STRIP_TAC >>
+(* We first prove that one iteration works *)
+subgoal `(weak_loop_step m ms wf_rel var l le invariant C1) <> {}`  >- (
+  SIMP_TAC std_ss [weak_loop_step_def, LET_DEF] >>
+  FULL_SIMP_TAC std_ss [abstract_loop_jgmt_def] >>
+  QSPECL_X_ASSUM ``!x. _`` [`var ms`] >>
+  FULL_SIMP_TAC std_ss [abstract_jgmt_def] >>
+  QSPECL_X_ASSUM ``!ms'. _`` [`ms`] >>
+  REV_FULL_SIMP_TAC std_ss [] >>
+  FULL_SIMP_TAC std_ss [GSYM pred_setTheory.MEMBER_NOT_EMPTY] >>
+  EXISTS_TAC ``ms'':'a`` >>
+  FULL_SIMP_TAC std_ss [pred_setTheory.SPECIFICATION]
+) >>
+FULL_SIMP_TAC std_ss [] >>
+
+Q.ABBREV_TAC `MS' = (weak_loop_step m ms wf_rel var l le invariant C1)` >>
+Q.ABBREV_TAC `ms' = CHOICE MS'` >>
+
+(* We prove that the invariant is preserved *)
+SUBGOAL_THEN ``(weak_loop_step m ms wf_rel var l le invariant C1) ms'`` ASSUME_TAC >- (
+  FULL_SIMP_TAC std_ss [Abbr `ms'`] >>
+  ASSUME_TAC (ISPEC ``MS':'a->bool`` pred_setTheory.CHOICE_DEF) >>
+  REV_FULL_SIMP_TAC std_ss [pred_setTheory.SPECIFICATION]
+) >>
+Q.SUBGOAL_THEN `invariant ms'` ASSUME_TAC >- (
+  FULL_SIMP_TAC std_ss [weak_loop_step_def, LET_DEF]
+) >>
+FULL_SIMP_TAC std_ss [] >>
+Q.SUBGOAL_THEN `(m.pc ms') = l` ASSUME_TAC >- (
+  FULL_SIMP_TAC std_ss [weak_loop_step_def, LET_DEF]
+) >>
+FULL_SIMP_TAC std_ss [] >>
+
+(* If we exit the loop *)
+Cases_on `~ (C1 ms')` >- (
+  (FULL_SIMP_TAC std_ss [weak_loop_step_def, LET_DEF]) >>
+  (FULL_SIMP_TAC std_ss [abstract_jgmt_def]) >>
+  QSPECL_X_ASSUM  ``!x. _`` [`ms'`] >>
+  (REV_FULL_SIMP_TAC std_ss []) >>
+  ASSUME_TAC (Q.SPECL [`m`] weak_comp_thm) >>
+  REV_FULL_SIMP_TAC std_ss [] >>
+  QSPECL_X_ASSUM ``!x. _`` [`ms`, `{l}`, `le`, `ms'`, `ms''`] >>
+  REV_FULL_SIMP_TAC (std_ss) [SINGLETONS_UNION_thm] >>
+  Q.SUBGOAL_THEN `l NOTIN le` (FULLSIMP_BY_THM std_ss) >- (
+    FULL_SIMP_TAC std_ss [abstract_loop_jgmt_def, pred_setTheory.IN_SING]
+  ) >>
+  METIS_TAC []
+) >> (
+  FULL_SIMP_TAC std_ss []
+) >> (
+  FULL_SIMP_TAC std_ss [weak_loop_step_def, LET_DEF]
+) >>
+ASSUME_TAC (Q.SPECL [`m`] weak_comp_thm) >>
+REV_FULL_SIMP_TAC std_ss [] >>
+QSPECL_X_ASSUM ``!x. _`` [`ms`, `{l}`, `le`, `ms'`, `ms''`] >>
+REV_FULL_SIMP_TAC (std_ss) [SINGLETONS_UNION_thm] >>
+  Q.SUBGOAL_THEN `l NOTIN le` (FULLSIMP_BY_THM std_ss) >- (
+    FULL_SIMP_TAC std_ss [abstract_loop_jgmt_def, pred_setTheory.IN_SING]
+  ) >>
+  METIS_TAC []
 );
 
 (* Now just some final touches to get the theorem in the exact shape we want *)
 val abstract_loop_rule_tmp_thm = MP loop_fun_ind_spec inductive_invariant;
 
+(* OLD:
+val invariant_rule_tmp_thm = 
+MP 
+(Q.SPEC `(\m ms wf_rel var l le invariant C1.
+weak_model m ==>
+WF wf_rel ==>
+abstract_loop_jgmt m l le invariant C1 wf_rel var ==>
+abstract_jgmt m l le (\ms. (invariant ms) /\ (~(C1 ms))) post ==>
+((invariant ms) /\ ((m.pc ms) = l) /\ (C1 ms)) ==>
+ (?ms'. ((m.weak ms le ms') /\ (post ms'))))` loop_fun_ind) inductive_invariant_thm;
+*)
+
 val abstract_loop_rule_thm = store_thm("abstract_loop_rule_thm",
   ``!m.
     weak_model m ==>
-    !l le invariant C1 var post.
-    abstract_loop_jgmt m l le invariant C1 var ==>
+    !l le invariant C1 wf_rel var post.
+    WF wf_rel ==>
+    abstract_loop_jgmt m l le invariant C1 wf_rel var ==>
     abstract_jgmt m l le (\ms. invariant ms /\ ~C1 ms) post ==>
     abstract_jgmt m l le invariant post``,
 
+
 metis_tac [abstract_jgmt_def, abstract_loop_rule_tmp_thm]
+(* OLD:
+REPEAT STRIP_TAC >>
+SIMP_TAC std_ss [abstract_jgmt_def] >>
+REPEAT STRIP_TAC >>
+ASSUME_TAC (Q.SPECL [`m`, `ms`, `wf_rel`, `var`, `l`, `le`, `invariant`, `C1`] invariant_rule_tmp_thm) >>
+FULL_SIMP_TAC std_ss [] >>
+REV_FULL_SIMP_TAC std_ss [] >>
+Cases_on `C1 ms` >- (
+  FULL_SIMP_TAC std_ss [] >>
+  Q.EXISTS_TAC `ms'`>>
+  FULL_SIMP_TAC std_ss []
+) >>
+FULL_SIMP_TAC std_ss [abstract_jgmt_def] 
+*)
 );
 
 val _ = export_theory();
